verify/BECv2.v
@@ -1,0 +1,184 @@
+From BusyCoq Require Import Individual62.
+Require Import Lia.
+Require Import ZArith.
+Require Import String.
+From BusyCoq Require Import BinaryCounter.
+
+Open Scope list.
+
+Module Eat2Digit.
+Section Eat2Digit.
+Hypothesis tm:TM.
+Hypothesis QL QR:Q.
+Hypothesis qL qR d1 w0 w1 w2:list Sym.
+Hypothesis a0 a1:N.
+Hypothesis n_init:nat.
+
+Notation "c -->* c'" := (c -[ tm ]->* c') (at level 40).
+Notation "c -->+ c'" := (c -[ tm ]->+ c') (at level 40).
+
+Notation "l <| r" :=
+  (l <{{QL}} qL *> r) (at level 30).
+
+Notation "l |> r" :=
+  (l <* qR {{QR}}> r) (at level 30).
+
+Definition L n := BinaryCounter_0 d1 n.
+
+Definition R n m := w0^^n *> w1 *> w2^^m *> const 0.
+
+Hypothesis LInc:
+  forall r n,
+    L n <| r -->+
+    L (N.succ n) |> r.
+
+Hypothesis RInc:
+  forall l n m,
+    l |> R (1+n) m -->+
+    l <| R n (1+m).
+
+Hypothesis ROv:
+  forall n m,
+    L ((n*2+a0)*2+a1) |> R 0 m -->+
+    L n <| R (3+m) 0.
+
+Lemma RIncs k n m:
+  L k |> R n m -->*
+  L (k+(N.of_nat n)) |> R 0 (n+m).
+Proof.
+  gen k m.
+  induction n; intros.
+  - finish.
+  - follow100 RInc.
+    follow100 LInc.
+    follow IHn.
+    finish.
+Qed.
+
+Definition config n :=
+  L (((N.of_nat n)*2+a0)*2+a1) |> R 0 (n*3+(N.to_nat (a0*2+a1))).
+
+Lemma BigStep n:
+  config n -->+
+  config (1+n).
+Proof.
+  unfold config.
+  follow10 ROv.
+  follow100 LInc.
+  follow RIncs.
+  finish.
+Qed.
+
+Hypothesis init:
+  c0 -->*
+  config n_init.
+
+Lemma nonhalt: ~halts tm c0.
+Proof.
+  apply multistep_nonhalt with (c':=config n_init).
+  1: apply init.
+  apply progress_nonhalt_simple.
+  intro i.
+  eexists.
+  apply BigStep.
+Qed.
+
+End Eat2Digit.
+
+Inductive Cert :=
+| cert1
+  (QL QR : Q)
+  (qL qR d1 w0 w1 w2 : list Sym)
+  (a0 a1 : N)
+  (n_init : nat).
+
+Ltac solve_cert cert :=
+match cert with
+  (cert1
+  ?QL ?QR
+  ?qL ?qR ?d1 ?w0 ?w1 ?w2
+  ?a0 ?a1
+  ?n_init) =>
+  eapply (nonhalt _
+    QL QR
+    qL qR d1 w0 w1 w2
+    a0 a1
+    n_init);
+  [ intros;
+    apply LInc_0;
+    try (execute_with_shift_rule || fail)
+  | try (execute_with_shift_rule || fail)
+  | intros;
+    unfold L;
+    repeat (rewrite BinaryCounter_0_d0' || rewrite BinaryCounter_0_d1');
+    try (execute_with_shift_rule || fail)
+  | unfold config,L,R,BinaryCounter_0; cbn;
+    try (solve_init || fail)
+  ]
+end.
+
+
+Definition tm0 := Eval compute in (TM_from_str "1LB0LE_0LC1LD_1RA1LC_1RC---_1RF1LE_0RA0RF").
+Lemma nonhalt0: ~halts tm0 c0.
+Proof.
+  solve_cert (cert1 E A [1;0] [0;0] [1] [1] [0] [1] 0 0 0).
+Qed.
+
+Definition tm1 := Eval compute in (TM_from_str "1LB0LE_0LC1LD_1RA1LC_1LC---_1RF1LE_0RA0RF").
+Lemma nonhalt1: ~halts tm1 c0.
+Proof.
+  solve_cert (cert1 E A [1;0] [0;0] [1] [1] [0] [1] 0 0 0).
+Qed.
+
+Definition tm2 := Eval compute in (TM_from_str "1LB1LE_0LC1LD_1RA1LC_1RC---_1RF0LE_0RF0RA").
+Lemma nonhalt2: ~halts tm2 c0.
+Proof.
+  solve_cert (cert1 E A [0;1] [0;0] [1] [1] [0] [1] 0 0 0).
+Qed.
+
+Definition tm3 := Eval compute in (TM_from_str "1LB1LE_0LC1LD_1RA1LC_1LC---_1RF0LE_0RF0RA").
+Lemma nonhalt3: ~halts tm3 c0.
+Proof.
+  solve_cert (cert1 E A [0;1] [0;0] [1] [1] [0] [1] 0 0 0).
+Qed.
+
+Definition tm4 := Eval compute in (TM_from_str "1RB1LA_0RC0RB_1LD0LA_0LE1LF_1RC1LE_---1LE").
+Lemma nonhalt4: ~halts tm4 c0.
+Proof.
+  solve_cert (cert1 A C [1;0] [0;0] [1] [1] [0] [1] 0 1 0).
+Qed.
+
+Definition tm5 := Eval compute in (TM_from_str "1RB1LA_0RC0RB_1LD0LA_0LE1LF_1RC1LE_---1RE").
+Lemma nonhalt5: ~halts tm5 c0.
+Proof.
+  solve_cert (cert1 A C [1;0] [0;0] [1] [1] [0] [1] 0 1 0).
+Qed.
+
+Definition tm6 := Eval compute in (TM_from_str "1LB1RA_1LC0LD_1RD---_0LE1LD_1RF1LE_0RA0RF").
+Lemma nonhalt6: ~halts tm6 c0.
+Proof.
+  solve_cert (cert1 E A [0] [0] [1] [1] [0] [1] 0 0 0).
+Qed.
+
+Definition tm7 := Eval compute in (TM_from_str "1LB1RA_1LC0LD_1RD---_1LE1LD_1RF0LE_0RF0RA").
+Lemma nonhalt7: ~halts tm7 c0.
+Proof.
+  solve_cert (cert1 E A [1] [0] [1] [1] [0] [1] 0 0 0).
+Qed.
+
+Definition tm8 := Eval compute in (TM_from_str "1LB1RA_1LC0LD_1LD---_0LE1LD_1RF1LE_0RA0RF").
+Lemma nonhalt8: ~halts tm8 c0.
+Proof.
+  solve_cert (cert1 E A [0] [0] [1] [1] [0] [1] 0 0 0).
+Qed.
+
+Definition tm9 := Eval compute in (TM_from_str "1LB1RA_1LC0LD_1LD---_0LE1LD_1RF1LE_0RA0RF").
+Lemma nonhalt9: ~halts tm9 c0.
+Proof.
+  solve_cert (cert1 E A [0] [0] [1] [1] [0] [1] 0 0 0).
+Qed.
+
+
+
+
+End Eat2Digit.
