verify/BECv3.v
@@ -1,0 +1,405 @@
+From BusyCoq Require Import Individual62.
+Require Import Lia.
+Require Import ZArith.
+Require Import String.
+From BusyCoq Require Import BinaryCounter.
+From BusyCoq Require Import BinaryCounterFull.
+
+Open Scope list.
+
+Module ShiftDigit.
+Section ShiftDigit.
+Hypothesis tm:TM.
+Hypothesis QL QR:Q.
+Hypothesis qL qR d1' w0 w1 w2:list Sym.
+Hypothesis k_init n_init:N.
+
+Notation "c -->* c'" := (c -[ tm ]->* c') (at level 40).
+Notation "c -->+ c'" := (c -[ tm ]->+ c') (at level 40).
+
+Notation "l <| r" :=
+  (l <{{QL}} qL *> r) (at level 30).
+
+Notation "l |> r" :=
+  (l <* qR {{QR}}> r) (at level 30).
+
+
+Definition d1:=[0]++d1'.
+Definition d0:=BinaryCounter.d0 d1.
+
+Definition LC n := BinaryCounter_0 d1 n.
+Definition LC0 n m := BinaryCounter d0 d1 (d1' *> BinaryCounter_0 d1 m) n.
+
+Definition R n m := w0^^n *> w1 *> w2^^m *> const 0.
+
+Hypothesis LInc:
+  forall l r n,
+    l <* d0 <* d1^^n <| r -->+
+    l <* d1 <* d0^^n |> r.
+
+Hypothesis LOv:
+  forall l r n,
+    l <* [0] <* d1' <* d1^^n <| r -->+
+    l <* d0^^(1+n) |> r.
+
+Hypothesis RInc:
+  forall l n m,
+    l |> R (1+n) m -->+
+    l <| R n (1+m).
+
+Hypothesis ROv:
+  forall l n m,
+    l <* d0 <* d1^^n |> R 0 m -->+
+    l <* d1' <* d0^^n |> R (1+m) 0.
+
+Lemma rotate_0 n r:
+  d0^^n *> d1 *> r =
+  [0] *> d0^^n *> d1' *> r.
+Proof.
+  unfold d0,d1.
+  cbn.
+  simpl_rotate.
+  rewrite List.repeat_cons.
+  reflexivity.
+Qed.
+
+Lemma LC_Inc:
+  forall r n,
+    LC n <| r -->+
+    LC (N.succ n) |> r.
+Proof.
+  intros.
+  apply LInc_0.
+  apply LInc.
+Qed.
+
+Lemma LC0_Inc:
+  forall r n m,
+    not_full n ->
+    LC0 n m <| r -->+
+    LC0 (Pos.succ n) m |> r.
+Proof.
+  introv Hnf.
+  apply BinaryCounter.LInc.
+  2: apply Hnf.
+  apply LInc.
+Qed.
+
+Lemma LC_Overflow_0 r n:
+  LC0 (pow2' n) N0 <| r -->+
+  LC N0 |> r.
+Proof.
+  intros.
+  unfold LC0.
+  rewrite Counter_pow2'.
+  replace (BinaryCounter_0 d1 0) with ([0] *> const 0) by solve_const0_eq.
+  follow10 LOv.
+  finish.
+  unfold d0.
+  rewrite lpow_all0.
+  - reflexivity.
+  - apply BinaryCounter.d0_all0.
+Qed.
+
+Lemma LC_Overflow r n m:
+  LC0 (pow2' n) (Npos m) <| r -->+
+  LC0 (pow2 (1+n+(ctz m))) (shr m (S (ctz m))) |> r.
+Proof.
+  intros.
+  unfold LC0.
+  rewrite Counter_pow2',Counter_pow2.
+  rewrite Counter_shr_S_ctz.
+  change (BinaryCounter.d0 d1) with d0.
+  rewrite rotate_0.
+  follow10 LOv.
+  simpl_tape.
+  finish.
+Qed.
+
+
+Lemma R_Overflow k m:
+  LC k |> R 0 m -->+
+  LC0 (pow2 (ctz (N.succ_pos k)))(shr (N.succ_pos k) (S (ctz (N.succ_pos k)))) |> R (1+m) 0.
+Proof.
+  unfold LC,LC0.
+  rewrite Counter_shr_S_ctzS.
+  rewrite Counter_pow2.
+  follow10 ROv.
+  finish.
+Qed.
+
+Lemma Inc0 k j n m (Hnf:not_full k):
+  LC0 k j |> R (1+n) m -->+
+  LC0 (Pos.succ k) j |> R n (1+m).
+Proof.
+  follow11 RInc.
+  apply LC0_Inc,Hnf.
+Qed.
+
+Lemma LC0_Incs k j n m:
+  LC0 k j |> R ((N.to_nat (rest k))+n) m -->*
+  LC0 (pow2' (log2 k)) j |> R n ((N.to_nat (rest k))+m).
+Proof.
+  remember (N.to_nat (rest k)) as r.
+  gen k j n m.
+  induction r; intros.
+  - assert (rest k = 0)%N as E by lia.
+    rewrite <-full_iff_rest in E.
+    rewrite full_iff_pow2' in E.
+    rewrite <-E.
+    finish.
+  - assert (rest k <> 0)%N as E by lia.
+    rewrite <-not_full_iff_rest in E.
+    follow100 (Inc0 k j (r+n) m E).
+    epose proof (IHr (Pos.succ k) _ _ _ (1+m)).
+    follow H.
+    rewrite not_full_log2_S; auto.
+    finish.
+Unshelve.
+  rewrite not_full_iff_rest in E.
+  pose proof (rest_S _ E) as H.
+  lia.
+Qed.
+
+Lemma rest_pow2_add1 k n:
+  N.to_nat (rest (pow2 k)) + (1+n) =
+  Pos.to_nat (pow2 k) + n.
+Proof.
+  pose proof (rest_pow2 k).
+  lia.
+Qed.
+
+Lemma LC0_Incs' k j n m:
+  LC0 (pow2 k) j |> R ((Pos.to_nat (pow2 k))+n) m -->*
+  LC0 (pow2' k) j <| R n ((Pos.to_nat (pow2 k))+m).
+Proof.
+  pose proof (LC0_Incs (pow2 k) j (1+n) m) as H.
+  rewrite rest_pow2_add1 in H.
+  rewrite log2_pow2 in H.
+  follow H.
+  follow100 RInc.
+  rewrite <-rest_pow2_add1.
+  finish.
+Qed.
+
+Definition v j i :=
+  ((N.succ_pos (j*2))*(pow2 i))%positive.
+
+Lemma v_S j i:
+  (v (Npos j) i =
+  (pow2 i)+(v (shr j (S (ctz j))) (1 + i + ctz j)))%positive.
+Proof.
+  unfold v.
+  replace (N.succ_pos (N.pos j*2)) with (Pos.succ (j*2))%positive by lia.
+  rewrite Pos.mul_succ_l.
+  f_equal.
+  gen i.
+  induction j; intros.
+  - cbn[shr].
+    cbn[ctz].
+    cbn[shr].
+    replace (1+i+0) with (S i) by lia.
+    cbn[pow2].
+    lia.
+  - cbn[shr].
+    cbn[ctz].
+    specialize (IHj i).
+    replace (1+i+S (ctz j)) with (S(1+i+ctz j)) by lia.
+    cbn[pow2].
+    lia.
+  - cbn.
+    do 2 f_equal.
+    lia.
+Qed.
+
+Lemma v_shrSctz_ctz n:
+  (v (shr n (S (ctz n))) (ctz n)) = n.
+Proof.
+  unfold v.
+  induction n.
+  - cbn. lia.
+  - cbn[shr].
+    cbn[ctz].
+    cbn[pow2].
+    lia.
+  - cbn. lia.
+Qed.
+
+Lemma LC0_Incs'' i j n m:
+  LC0 (pow2 i) j |> R ((Pos.to_nat (v j i))+n) m -->*
+  LC 0 |> R n ((Pos.to_nat (v j i))+m).
+Proof.
+  gen i n m.
+  induction j using N_strong_induction.
+  intros.
+  destruct j as [|j].
+  - unfold v.
+    cbn[N.mul].
+    cbn[N.succ_pos].
+    cbn[Pos.mul].
+    follow LC0_Incs'.
+    follow100 LC_Overflow_0.
+    finish.
+  - rewrite v_S.
+    rewrite Pos2Nat.inj_add.
+    repeat rewrite <-Nat.add_assoc.
+    follow LC0_Incs'.
+    follow100 LC_Overflow.
+    epose proof (H (shr j (S (ctz j))) _ (1+i+ctz j)) as H0.
+    follow H0.
+    repeat rewrite Nat.add_assoc.
+    finish.
+Unshelve.
+  apply shr_S_lt.
+Qed.
+
+Lemma Incs k n m:
+  LC k |> R n m -->*
+  LC (k+(N.of_nat n)) |> R 0 (n+m).
+Proof.
+  gen k m.
+  induction n; intros.
+  - finish.
+  - follow100 RInc.
+    follow100 LC_Inc.
+    follow IHn.
+    finish.
+Qed.
+
+Lemma BigStep k m:
+  LC k |> R 0 ((N.to_nat k)+m) -->+ LC (N.of_nat m) |> R 0 ((N.to_nat k)+m+1).
+Proof.
+  follow10 R_Overflow.
+  remember (N.succ_pos k) as k'.
+  epose proof (LC0_Incs'' (ctz k') (shr k' (S (ctz k'))) m 0).
+  rewrite v_shrSctz_ctz in H.
+  replace (1+((N.to_nat k) + m)) with (Pos.to_nat k' + m) by lia.
+  follow H.
+  follow Incs.
+  finish.
+Qed.
+
+Inductive Config:=
+| cfg0 (k n:N)
+| cfg1 (k n:N)
+.
+
+Definition to_config(x:Config):=
+match x with
+| cfg0 k n => LC k |> R 0 ((N.to_nat (k+n)))
+| cfg1 k n => LC n |> R 0 ((N.to_nat (k+n+1)))
+end.
+
+Hypothesis init:
+  c0 -->*
+  to_config (cfg0 k_init n_init).
+
+Lemma nonhalt: ~halts tm c0.
+Proof.
+  eapply multistep_nonhalt.
+  1: apply init.
+  apply progress_nonhalt_simple.
+  intro i.
+  destruct i as [k|k].
+  - exists (cfg1 k n).
+    cbn[to_config].
+    replace (N.to_nat (k+n)) with (N.to_nat k + N.to_nat n) by lia.
+    follow10 BigStep.
+    finish.
+  - exists (cfg0 (N.succ k) (N.succ n)).
+    cbn[to_config].
+    replace (N.to_nat (k+n+1)) with (N.to_nat n + (N.to_nat k + 1)) by lia.
+    follow10 BigStep.
+    finish.
+Qed.
+
+End ShiftDigit.
+
+Inductive Cert :=
+| cert1
+  (QL QR : Q)
+  (qL qR d1' w0 w1 w2 : list Sym)
+  (k_init n_init : N).
+
+Ltac solve_cert cert :=
+match cert with
+  (cert1
+  ?QL ?QR
+  ?qL ?qR ?d1' ?w0 ?w1 ?w2
+  ?k_init ?n_init) =>
+  eapply (nonhalt _
+    QL QR
+    qL qR d1' w0 w1 w2
+    k_init n_init);
+  [ unfold d0,d1;
+    try (execute_with_shift_rule; fail)
+  | unfold d0,d1;
+    try (execute_with_shift_rule; fail)
+  | unfold R;
+    try (execute_with_shift_rule; fail)
+  | unfold d0,d1,R;
+    try (execute_with_shift_rule; fail)
+  | cbn;
+    try (solve_init; fail)
+  ]
+end.
+
+
+Definition tm0 := Eval compute in (TM_from_str "1LB0RA_1RC1LE_1LD1RD_0LB1LA_0LB0LF_0LB---").
+Lemma nonhalt0: ~halts tm0 c0.
+Proof.
+  solve_cert (cert1 E D [1;0] [1;1] [0;0;1] [1;0] [0] [1;0] 0 0).
+Qed.
+
+Definition tm1 := Eval compute in (TM_from_str "1LB0RA_1RC1LE_1LD1RD_0LE1LA_0LB0LF_---0RC").
+Lemma nonhalt1: ~halts tm1 c0.
+Proof.
+  solve_cert (cert1 E D [1;0] [1;1] [0;0;1] [1;0] [0] [1;0] 0 0).
+Qed.
+
+Definition tm2 := Eval compute in (TM_from_str "1LB1RB_0LC1LD_1RA1LE_1LC0RD_0LC0LF_0LC---").
+Lemma nonhalt2: ~halts tm2 c0.
+Proof.
+  solve_cert (cert1 E B [1;0] [1;1] [0;0;1] [1;0] [0] [1;0] 2 0).
+Qed.
+
+Definition tm3 := Eval compute in (TM_from_str "1LB1RB_0LC1LE_0LD1LF_1RA1LC_1LD0RE_---0LC").
+Lemma nonhalt3: ~halts tm3 c0.
+Proof.
+  solve_cert (cert1 C B [1;0] [1;1] [0;0;1] [1;0] [0] [1;0] 1 1).
+Qed.
+
+Definition tm4 := Eval compute in (TM_from_str "1RB1LE_1LC1RC_0LA1LD_1LA0RD_0LA0LF_0LA---").
+Lemma nonhalt4: ~halts tm4 c0.
+Proof.
+  solve_cert (cert1 E C [1;0] [1;1] [0;0;1] [1;0] [0] [1;0] 1 0).
+Qed.
+
+Definition tm5 := Eval compute in (TM_from_str "1RB1LE_1LC1RC_0LE1LD_1LA0RD_0LA0LF_---0RB").
+Lemma nonhalt5: ~halts tm5 c0.
+Proof.
+  solve_cert (cert1 E C [1;0] [1;1] [0;0;1] [1;0] [0] [1;0] 1 0).
+Qed.
+
+Definition tm6 := Eval compute in (TM_from_str "1RB1LE_1LC1RC_0LE1LD_1LA0RD_0LA1LF_---0LE").
+Lemma nonhalt6: ~halts tm6 c0.
+Proof.
+  solve_cert (cert1 E C [1;0] [1;1] [0;0;1] [1;0] [0] [1;0] 1 0).
+Qed.
+
+Definition tm7 := Eval compute in (TM_from_str "1LB0LC_1LC0RD_1RD1LA_0LE0RD_1RC1LF_---0LA").
+Lemma nonhalt7: ~halts tm7 c0.
+Proof.
+  solve_cert (cert1 A D [1;0] [1;1] [0;1] [1;0] [0] [1;0] 1 0).
+Qed.
+
+Definition tm8 := Eval compute in (TM_from_str "1RB1LD_1RC1LE_0LA0RC_---0LE_1LF0LB_1LB0RC").
+Lemma nonhalt8: ~halts tm8 c0.
+Proof.
+  solve_cert (cert1 E C [1;0] [1;1] [0;1] [1;0] [0] [1;0] 1 1).
+Qed.
+
+
+
+
+End ShiftDigit.
