verify/SOBCv1.v
@@ -1,0 +1,922 @@
+From BusyCoq Require Import Individual62.
+Require Import Lia.
+Require Import ZArith.
+Require Import String.
+From BusyCoq Require Import BinaryCounter.
+From BusyCoq Require Import BinaryCounterFull.
+
+Open Scope list.
+
+Section SOBCv1.
+
+Hypothesis tm:TM.
+Hypothesis QL QR:Q.
+Hypothesis qL qR:list Sym.
+Hypothesis n_init m_init:nat.
+
+Notation "c -->* c'" := (c -[ tm ]->* c') (at level 40).
+Notation "c -->+ c'" := (c -[ tm ]->+ c') (at level 40).
+
+Notation "l <| r" :=
+  (l <{{QL}} qL *> r) (at level 30).
+
+Notation "l |> r" :=
+  (l <* qR {{QR}}> r) (at level 30).
+
+
+Definition d0 := [0;0;1].
+Definition d1 := [1;1;1].
+Definition d1a := [1;1] *> const 0.
+
+Definition L n := BinaryCounter d0 d1 d1a n.
+Definition R n := [1]^^n *> const 0.
+
+Hypothesis HLInc:
+  forall (l r0 : side) (n0 : nat), d1 ^^ n0 *> d0 *> l <| r0 -->+ d0 ^^ n0 *> d1 *> l |> r0.
+
+Lemma LInc:
+  forall r n (Hnf:not_full n),
+    L n <| r -->+
+    L (Pos.succ n) |> r.
+Proof.
+  intros.
+  apply LInc.
+  - apply HLInc.
+  - apply Hnf.
+Qed.
+
+Hypothesis RInc:
+  forall l n,
+    l |> R (n*2) -->+
+    l <| R (2+n*2).
+
+Hypothesis HLOv2:
+  forall n m,
+  d1 ^^ n *> d1a <| [1] ^^ (2 + m * 3) *> const 0 -->+
+  d0 ^^ (1 + m) *> d1 *> d0 ^^ n *> d1a <| [1] ^^ 0 *> const 0.
+
+Lemma LOv2 n m:
+  L (pow2' n) <| R (2+m*3) -->+
+  L (((pow2 n)~1)*(pow2 (1+m))) <| R 0.
+Proof.
+  unfold L,R.
+  rewrite Counter_pow2'.
+  rewrite Counter_mulpow2.
+  cbn[BinaryCounter].
+  rewrite Counter_pow2.
+  apply HLOv2.
+Qed.
+
+Lemma LIncs n m:
+  L n <| R (m*2) -->*
+  L (pow2' (log2 n)) <| R ((N.to_nat (rest n))*2+m*2).
+Proof.
+  remember (N.to_nat (rest n)) as r.
+  gen n m.
+  induction r; intros.
+  - assert (rest n = 0)%N as E by lia.
+    rewrite <-full_iff_rest in E.
+    rewrite full_iff_pow2' in E.
+    rewrite <-E.
+    finish.
+  - assert (rest n <> 0)%N as E by lia.
+    pose proof (rest_S _ E) as H.
+    rewrite <-not_full_iff_rest in E.
+    follow100 (LInc (R (m*2)) _ E).
+    follow100 RInc.
+    epose proof (IHr (Pos.succ n) _ (1+m)) as H1.
+    follow H1.
+    rewrite not_full_log2_S. 2: apply E.
+    finish.
+Unshelve.
+  lia.
+Qed.
+
+Lemma BigStep2 n m:
+  L (pow2' n) <| R (2+m*6) -->+
+  L (pow2' (2+m*2+n)) <| R (N.to_nat ((((N.pos (pow2 n))*2-1)*(N.pos (pow2 (1+m*2)))-1)*2)).
+Proof.
+  replace (m*6) with ((m*2)*3) by lia.
+  follow10 LOv2.
+  epose proof (LIncs _ 0) as H'.
+  follow H'.
+  clear H'.
+  rewrite log2_mulpow2.
+  cbn[log2].
+  rewrite log2_pow2.
+  pose proof (rest_mul_pow2 ((pow2 n)~1) (1+m*2)) as H.
+  rewrite rest_mul2add1 in H.
+  pose proof (rest_pow2 n) as H0.
+  finish.
+Qed.
+
+Lemma pow2_mul2_mod3 n:
+  (N.pos (pow2 (n*2)) mod 3 = 1)%N.
+Proof.
+  induction n.
+  - reflexivity.
+  - cbn.
+    replace (N.pos (pow2 (n * 2))~0~0) with ((N.pos (pow2 (n*2)))*4)%N by lia.
+    rewrite N.Div0.mul_mod.
+    rewrite IHn.
+    reflexivity.
+Qed.
+
+Lemma sub_mod a b c:
+  (a>=b ->
+  c<>0 ->
+  ((a-b) mod c) =
+  ((a mod c)+(c-(b mod c))) mod c)%N.
+Proof.
+  intros H H0.
+  remember (a-b)%N as d.
+  replace a with (d+b)%N by lia.
+  rewrite N.Div0.add_mod_idemp_l.
+  pose proof (N.mod_upper_bound b c H0).
+  pose proof (N.Div0.mod_le b c).
+  replace (d+b+(c-b mod c))%N with (b+(d+c-(b mod c)))%N by lia.
+  rewrite <-N.Div0.add_mod_idemp_l.
+  replace (b mod c+(d+c-(b mod c)))%N with (d+c)%N by lia.
+  rewrite <-N.Div0.add_mod_idemp_r.
+  rewrite N.Div0.mod_same.
+  rewrite N.add_0_r.
+  reflexivity.
+Qed.
+
+Lemma Npos_mul a b:
+  Npos (a*b)%positive = ((N.pos a)*(N.pos b))%N.
+Proof.
+  lia.
+Qed.
+
+Lemma BigStep n m:
+  L (pow2' (n*2)) <| R (2+m*6) -->+
+  L (pow2' ((1+m+n)*2)) <| R (N.to_nat (2+((((N.pos (pow2 (n*2)))*2-1)*(N.pos (pow2 (1+m*2)))-2)/3) * 6)).
+Proof.
+  follow10 BigStep2.
+  remember (N.pos (pow2 (n * 2)) * 2 - 1)%N as v1.
+  change (pow2 (1+m*2))%positive with (2*(pow2 (m*2)))%positive.
+  remember (N.pos (2 * pow2 (m * 2))) as v2.
+  assert (v1>=1)%N as E1 by lia.
+  assert (v2>=2)%N as E2 by lia.
+  replace (v1*v2-1)%N with (v1*v2-2+1)%N by lia.
+  rewrite N.mul_add_distr_r.
+  assert ((v1*v2-2) mod 3 = 0)%N. {
+    rewrite sub_mod. 2,3: lia. cbn.
+    rewrite N.Div0.mul_mod.
+    rewrite Heqv2,Heqv1.
+    repeat rewrite Npos_mul.
+    rewrite sub_mod. 2,3: lia.
+    rewrite (N.Div0.mul_mod (N.pos (pow2 (n * 2)))).
+    rewrite (N.Div0.mul_mod _ (N.pos (pow2 (m * 2)))).
+    repeat rewrite pow2_mul2_mod3.
+    reflexivity.
+  }
+  finish.
+Qed.
+
+Definition config (x:nat*nat) :=
+  let (n,m):=x in
+  L (pow2' (n*2)) <| R (2+m*6).
+
+
+Hypothesis init:
+  c0 -->*
+  config (n_init,m_init)%nat.
+
+Lemma nonhalt: ~halts tm c0.
+Proof.
+  eapply multistep_nonhalt with (c':=config _).
+  1: apply init.
+  apply progress_nonhalt_simple.
+  intro i.
+  destruct i as [n m].
+  eexists (_,_).
+  cbn[config].
+  follow10 BigStep.
+  rewrite Nnat.N2Nat.inj_add.
+  rewrite Nnat.N2Nat.inj_mul.
+  finish.
+Qed.
+
+End SOBCv1.
+
+Inductive Cert :=
+| cert1
+  (QL QR : Q)
+  (qL qR : list Sym)
+  (n_init m_init : nat).
+
+Ltac solve_cert cert :=
+match cert with
+  (cert1
+  ?QL ?QR
+  ?qL ?qR
+  ?n_init ?m_init) =>
+  eapply (nonhalt _
+    QL QR
+    qL qR
+    n_init m_init);
+  [ unfold d0,d1,d1a;
+    try (execute_with_shift_rule || fail)
+  | intros;
+    unfold R;
+    simpl_tape;
+    repeat rewrite lpow_mul;
+    try (execute_with_shift_rule || fail)
+  | intros;
+    simpl_tape;
+    rewrite lpow_mul;
+    unfold d0,d1,d1a;
+    try (execute_with_shift_rule || fail)
+  | unfold config; cbn;
+    try (solve_init || fail)
+  ]
+end.
+
+Definition tm0 := Eval compute in (TM_from_str "1RB0RB_0RC0LE_1LD0RD_1LA0RF_1LD1RA_---0LA").
+Lemma nonhalt0: ~halts tm0 c0.
+Proof.
+  solve_cert (cert1 D B [1;0;1;0] [1;1;0;1] 0 0).
+Qed.
+
+Definition tm1 := Eval compute in (TM_from_str "1LB0LB_1RC1LE_0RA0RD_1LE0RE_0LB0RF_---0LC").
+Lemma nonhalt1: ~halts tm1 c0.
+Proof.
+  solve_cert (cert1 E A [1;0;1;0] [0;1;0;1] 0 0).
+Qed.
+
+Definition tm2 := Eval compute in (TM_from_str "1RB1RB_1LC0LE_1LF1RD_---0RE_1LC0RC_1RA0RB").
+Lemma nonhalt2: ~halts tm2 c0.
+Proof.
+  solve_cert (cert1 C B [1;0;1;0] [1;1;0;1] 0 0).
+Qed.
+
+Definition tm3 := Eval compute in (TM_from_str "1RB0RC_0LB1RC_1LD0LF_1LA1RE_---0RF_1LD0RD").
+Lemma nonhalt3: ~halts tm3 c0.
+Proof.
+  solve_cert (cert1 D C [1;0;1;0] [1;1;0;1] 0 0).
+Qed.
+
+Definition tm4 := Eval compute in (TM_from_str "1RB0RC_0RC1RC_1LD0LE_1LA1RF_1LD0RD_---0RE").
+Lemma nonhalt4: ~halts tm4 c0.
+Proof.
+  solve_cert (cert1 D C [1;0;1;0] [1;1;0;1] 0 0).
+Qed.
+
+Definition tm5 := Eval compute in (TM_from_str "1RB0RC_1LC1RC_1LE0LD_1LE0RE_1LA1RF_---0RD").
+Lemma nonhalt5: ~halts tm5 c0.
+Proof.
+  solve_cert (cert1 E C [1;0;1;0] [1;1;0;1] 0 0).
+Qed.
+
+Definition tm6 := Eval compute in (TM_from_str "1RB0RD_1RC1RD_1LA1RF_1LC0LE_1LC0RC_---0RE").
+Lemma nonhalt6: ~halts tm6 c0.
+Proof.
+  solve_cert (cert1 C D [1;0;1;0] [1;1;0;1] 0 0).
+Qed.
+
+Definition tm7 := Eval compute in (TM_from_str "1RB0RE_0RC1RB_1LD0RD_1LA1RF_0LA0LC_---0LA").
+Lemma nonhalt7: ~halts tm7 c0.
+Proof.
+  solve_cert (cert1 D B [1;0;1;0] [1;1;0;1] 0 0).
+Qed.
+
+Definition tm8 := Eval compute in (TM_from_str "1RB0RE_0RC1RE_1LD0RD_1LA1RF_0LA0LC_---0RC").
+Lemma nonhalt8: ~halts tm8 c0.
+Proof.
+  solve_cert (cert1 D E [1;0;1;0] [1;1;0;1] 0 0).
+Qed.
+
+Definition tm9 := Eval compute in (TM_from_str "1RB0RE_0RC1RE_1LD0RD_1LA1RF_1LD0LC_---0RC").
+Lemma nonhalt9: ~halts tm9 c0.
+Proof.
+  solve_cert (cert1 D E [1;0;1;0] [1;1;0;1] 0 0).
+Qed.
+
+Definition tm10 := Eval compute in (TM_from_str "1RB1RE_0RC1RB_1LD0RD_1LA0RE_0LF0LA_---1LD").
+Lemma nonhalt10: ~halts tm10 c0.
+Proof.
+  solve_cert (cert1 D B [1;0;1;0] [1;1;0;1] 0 0).
+Qed.
+
+Definition tm11 := Eval compute in (TM_from_str "1RB0RF_1LC0LF_0LE0RD_---1LE_1RA1LC_1LC0RC").
+Lemma nonhalt11: ~halts tm11 c0.
+Proof.
+  solve_cert (cert1 C B [1;0;1;0] [1;1;0;1] 0 0).
+Qed.
+
+Definition tm12 := Eval compute in (TM_from_str "1RB0RF_1LC1RF_1LA1RD_---0RE_1LC0RC_0LA0LE").
+Lemma nonhalt12: ~halts tm12 c0.
+Proof.
+  solve_cert (cert1 C F [1;0;1;0] [1;1;0;1] 0 0).
+Qed.
+
+Definition tm13 := Eval compute in (TM_from_str "1RB0RF_1LC1RF_1LA1RD_---0RE_1LC0RC_1LC0LE").
+Lemma nonhalt13: ~halts tm13 c0.
+Proof.
+  solve_cert (cert1 C F [1;0;1;0] [1;1;0;1] 0 0).
+Qed.
+
+Definition tm14 := Eval compute in (TM_from_str "1RB1RF_1LC0RC_1LE1RD_---0RB_1RA0RF_1LC0LB").
+Lemma nonhalt14: ~halts tm14 c0.
+Proof.
+  solve_cert (cert1 C F [1;0;1;0] [1;1;0;1] 0 0).
+Qed.
+
+Definition tm15 := Eval compute in (TM_from_str "1RB---_0RC0LC_1LD0RD_0LE0RF_1RA1LD_---0LA").
+Lemma nonhalt15: ~halts tm15 c0.
+Proof.
+  solve_cert (cert1 D B [1;0;1;0] [1;1;0;1] 0 0).
+Qed.
+
+Definition tm16 := Eval compute in (TM_from_str "1RB1RB_0RC0LC_1LD0RD_0LE1RF_1RA1LD_---0LA").
+Lemma nonhalt16: ~halts tm16 c0.
+Proof.
+  solve_cert (cert1 D B [1;0;1;0] [1;1;0;1] 0 0).
+Qed.
+
+Definition tm17 := Eval compute in (TM_from_str "1RB1RB_0RC0LC_1LD0RD_1LE1RF_1RA0RB_---0RC").
+Lemma nonhalt17: ~halts tm17 c0.
+Proof.
+  solve_cert (cert1 D B [1;0;1;0] [1;1;0;1] 0 0).
+Qed.
+
+Definition tm18 := Eval compute in (TM_from_str "1RB0RC_0LB1RC_0RD0LD_1LE0RE_1LA1RF_---0RD").
+Lemma nonhalt18: ~halts tm18 c0.
+Proof.
+  solve_cert (cert1 E C [1;0;1;0] [1;1;0;1] 0 0).
+Qed.
+
+Definition tm19 := Eval compute in (TM_from_str "1RB0RC_0RC0LC_1LD0RD_0LE0RF_1RA1LD_---1LE").
+Lemma nonhalt19: ~halts tm19 c0.
+Proof.
+  solve_cert (cert1 D B [1;0;1;0] [1;1;0;1] 0 0).
+Qed.
+
+Definition tm20 := Eval compute in (TM_from_str "1RB0RC_1LC1RC_0RD0LD_1LE0RE_1LA1RF_---0RD").
+Lemma nonhalt20: ~halts tm20 c0.
+Proof.
+  solve_cert (cert1 E C [1;0;1;0] [1;1;0;1] 0 0).
+Qed.
+
+Definition tm21 := Eval compute in (TM_from_str "1RB0RD_0RC0LA_1LD0RD_0LE0RF_1RA1LD_---0LA").
+Lemma nonhalt21: ~halts tm21 c0.
+Proof.
+  solve_cert (cert1 D B [1;0;1;0] [1;1;0;1] 0 0).
+Qed.
+
+Definition tm22 := Eval compute in (TM_from_str "1RB0RD_1RC1RD_1LA1RF_0RE0LE_1LC0RC_---0RE").
+Lemma nonhalt22: ~halts tm22 c0.
+Proof.
+  solve_cert (cert1 C D [1;0;1;0] [1;1;0;1] 0 0).
+Qed.
+
+Definition tm23 := Eval compute in (TM_from_str "1RB0RE_0RC1RE_1LD0RD_1LA1RF_0RC0LC_---0RC").
+Lemma nonhalt23: ~halts tm23 c0.
+Proof.
+  solve_cert (cert1 D E [1;0;1;0] [1;1;0;1] 0 0).
+Qed.
+
+Definition tm24 := Eval compute in (TM_from_str "1RB1RE_0RC0LF_1LD0RD_0LE0RF_1RA1LD_---0LA").
+Lemma nonhalt24: ~halts tm24 c0.
+Proof.
+  solve_cert (cert1 D B [1;0;1;0] [1;1;0;1] 0 0).
+Qed.
+
+Definition tm25 := Eval compute in (TM_from_str "1RB0RF_1LC1RF_1LA1RD_---0RE_1LC0RC_0RE0LE").
+Lemma nonhalt25: ~halts tm25 c0.
+Proof.
+  solve_cert (cert1 C F [1;0;1;0] [1;1;0;1] 0 0).
+Qed.
+
+Definition tm26 := Eval compute in (TM_from_str "1RB1RF_1LC0RC_1LE1RD_---0RB_1RA0RF_0RB0LB").
+Lemma nonhalt26: ~halts tm26 c0.
+Proof.
+  solve_cert (cert1 C F [1;0;1;0] [1;1;0;1] 0 0).
+Qed.
+
+Definition tm27 := Eval compute in (TM_from_str "1RB0RE_1LC0LF_1LA1RD_---0RB_0RC0LB_0RE1RA").
+Lemma nonhalt27: ~halts tm27 c0.
+Proof.
+  solve_cert (cert1 C B [1;0;1;0] [1;1;0;1] 0 0).
+Qed.
+
+Definition tm28 := Eval compute in (TM_from_str "1RB0RE_1LC0LF_1LA1RD_---0RB_0RC0LB_1LF1RA").
+Lemma nonhalt28: ~halts tm28 c0.
+Proof.
+  solve_cert (cert1 C B [1;0;1;0] [1;1;0;1] 0 0).
+Qed.
+
+Definition tm29 := Eval compute in (TM_from_str "1RB1RE_0RC1RB_1LD0RD_1LA0RE_0LF0LA_---0LB").
+Lemma nonhalt29: ~halts tm29 c0.
+Proof.
+  solve_cert (cert1 B B [0;0;1;0] [1;1;0;1] 0 0).
+Qed.
+
+Definition tm30 := Eval compute in (TM_from_str "1RB1RE_0RC1RB_1LD0RD_1LA1RF_0LF0LA_---0LB").
+Lemma nonhalt30: ~halts tm30 c0.
+Proof.
+  solve_cert (cert1 B B [0;0;1;0] [1;1;0;1] 0 0).
+Qed.
+
+Definition tm31 := Eval compute in (TM_from_str "1RB---_0RC0LC_1LD0RD_0LE1RF_1RA1LD_---0RC").
+Lemma nonhalt31: ~halts tm31 c0.
+Proof.
+  solve_cert (cert1 D B [1;0;1;0] [1;1;0;1] 0 0).
+Qed.
+
+Definition tm33 := Eval compute in (TM_from_str "1RB---_1LC0LE_0LF1RD_---0RE_1LC0RC_1RA1LC").
+Lemma nonhalt33: ~halts tm33 c0.
+Proof.
+  solve_cert (cert1 C B [1;0;1;0] [1;1;0;1] 0 0).
+Qed.
+
+Definition tm34 := Eval compute in (TM_from_str "1RB1RA_0RC0LA_1LD0RD_0LE0RF_1RA1LD_---0LA").
+Lemma nonhalt34: ~halts tm34 c0.
+Proof.
+  solve_cert (cert1 D B [1;0;1;0] [1;1;0;1] 0 0).
+Qed.
+
+Definition tm35 := Eval compute in (TM_from_str "1RB0LB_0RC1RB_1LD0RD_0LE0RF_1RA1LD_---1LE").
+Lemma nonhalt35: ~halts tm35 c0.
+Proof.
+  solve_cert (cert1 D B [1;0;1;0] [1;1;0;1] 0 0).
+Qed.
+
+Definition tm36 := Eval compute in (TM_from_str "1RB0LB_1LC0RC_1LE0RD_---0LE_1RF0RA_0RB1RF").
+Lemma nonhalt36: ~halts tm36 c0.
+Proof.
+  solve_cert (cert1 C F [1;0;1;0] [1;1;0;1] 0 0).
+Qed.
+
+Definition tm37 := Eval compute in (TM_from_str "1RB0LB_1LC0RC_1LF1RD_---0LE_0RB1RE_1RE0RA").
+Lemma nonhalt37: ~halts tm37 c0.
+Proof.
+  solve_cert (cert1 C E [1;0;1;0] [1;1;0;1] 0 0).
+Qed.
+
+Definition tm38 := Eval compute in (TM_from_str "1RB0RB_0RC0LE_1LD0RD_1LA1RF_1LD1RA_---0RC").
+Lemma nonhalt38: ~halts tm38 c0.
+Proof.
+  solve_cert (cert1 D B [1;0;1;0] [1;1;0;1] 0 0).
+Qed.
+
+Definition tm39 := Eval compute in (TM_from_str "1LB0LB_1RC1LE_0RA0RD_1LE0RE_0LB0RF_---1LB").
+Lemma nonhalt39: ~halts tm39 c0.
+Proof.
+  solve_cert (cert1 E A [1;0;1;0] [0;1;0;1] 0 0).
+Qed.
+
+Definition tm40 := Eval compute in (TM_from_str "1RB0RB_1LC0LF_1LA1RD_---0RE_1LC0RC_1LC1RA").
+Lemma nonhalt40: ~halts tm40 c0.
+Proof.
+  solve_cert (cert1 C B [1;0;1;0] [1;1;0;1] 0 0).
+Qed.
+
+Definition tm41 := Eval compute in (TM_from_str "1RB0LC_0RC1RB_1LD0RD_1LE0RF_1RB0RA_---0LA").
+Lemma nonhalt41: ~halts tm41 c0.
+Proof.
+  solve_cert (cert1 D B [1;0;1;0] [1;1;0;1] 0 0).
+Qed.
+
+Definition tm42 := Eval compute in (TM_from_str "1RB0LC_0RC1RB_1LD0RD_1LE0RF_1RB0RA_---0LE").
+Lemma nonhalt42: ~halts tm42 c0.
+Proof.
+  solve_cert (cert1 D B [1;0;1;0] [1;1;0;1] 0 0).
+Qed.
+
+Definition tm43 := Eval compute in (TM_from_str "1RB0LC_0RC1RB_1LD0RD_1LE1RF_1RB0RA_---0LB").
+Lemma nonhalt43: ~halts tm43 c0.
+Proof.
+  solve_cert (cert1 D B [1;0;1;0] [1;1;0;1] 0 0).
+Qed.
+
+Definition tm44 := Eval compute in (TM_from_str "1RB0RC_1LC0LA_0LF1RD_---0RE_1LC0RC_1RA1LC").
+Lemma nonhalt44: ~halts tm44 c0.
+Proof.
+  solve_cert (cert1 C B [1;0;1;0] [1;1;0;1] 0 0).
+Qed.
+
+Definition tm45 := Eval compute in (TM_from_str "1RB1RC_0LA0LC_1LD0RD_0LF1RE_---0RC_1RA1LD").
+Lemma nonhalt45: ~halts tm45 c0.
+Proof.
+  solve_cert (cert1 D B [1;0;1;0] [1;1;0;1] 0 0).
+Qed.
+
+Definition tm46 := Eval compute in (TM_from_str "1RB1RC_1LA0LD_---0RD_1LE0RE_0LF1RC_1RA1LE").
+Lemma nonhalt46: ~halts tm46 c0.
+Proof.
+  solve_cert (cert1 E B [1;0;1;0] [1;1;0;1] 0 0).
+Qed.
+
+Definition tm47 := Eval compute in (TM_from_str "1RB1RC_1LA0LF_1RA1LD_0LC1RE_---0RF_1LD0RD").
+Lemma nonhalt47: ~halts tm47 c0.
+Proof.
+  solve_cert (cert1 D B [1;0;1;0] [1;1;0;1] 0 0).
+Qed.
+
+Definition tm48 := Eval compute in (TM_from_str "1RB0RD_0RC0LA_1LD0RD_0LE1RF_1RA1LD_---0RC").
+Lemma nonhalt48: ~halts tm48 c0.
+Proof.
+  solve_cert (cert1 D B [1;0;1;0] [1;1;0;1] 0 0).
+Qed.
+
+Definition tm49 := Eval compute in (TM_from_str "1RB0RD_1LC1RE_1LA1RD_---0LB_0RF1RB_1LC0RC").
+Lemma nonhalt49: ~halts tm49 c0.
+Proof.
+  solve_cert (cert1 C E [1;0;1;0] [1;1;0;1] 0 0).
+Qed.
+
+Definition tm50 := Eval compute in (TM_from_str "1RB0RD_1LC1RE_1LA1RD_---0LB_0RF1RE_1LC0RC").
+Lemma nonhalt50: ~halts tm50 c0.
+Proof.
+  solve_cert (cert1 C E [1;0;1;0] [1;1;0;1] 0 0).
+Qed.
+
+Definition tm51 := Eval compute in (TM_from_str "1RB1LD_0RC1RB_1LD0RD_1LE0RF_1RB1RF_---0LA").
+Lemma nonhalt51: ~halts tm51 c0.
+Proof.
+  solve_cert (cert1 D B [1;0;1;0] [1;1;0;1] 0 0).
+Qed.
+
+Definition tm52 := Eval compute in (TM_from_str "1RB0RE_0RC1RB_1LD0RD_1LA1RE_---0LF_1LD1RB").
+Lemma nonhalt52: ~halts tm52 c0.
+Proof.
+  solve_cert (cert1 D B [1;0;1;0] [1;1;0;1] 0 0).
+Qed.
+
+Definition tm53 := Eval compute in (TM_from_str "1RB0RE_0RC1RB_1LD0RD_1LA0RF_---0LC_---0LA").
+Lemma nonhalt53: ~halts tm53 c0.
+Proof.
+  solve_cert (cert1 D B [1;0;1;0] [1;1;0;1] 0 0).
+Qed.
+
+Definition tm54 := Eval compute in (TM_from_str "1RB0RE_0RC1RB_1LD0RD_1LA0RF_1LD0LE_---0LA").
+Lemma nonhalt54: ~halts tm54 c0.
+Proof.
+  solve_cert (cert1 D B [1;0;1;0] [1;1;0;1] 0 0).
+Qed.
+
+Definition tm55 := Eval compute in (TM_from_str "1RB0RE_0RC1RB_1LD0RD_1LA1RF_---0LC_---0LB").
+Lemma nonhalt55: ~halts tm55 c0.
+Proof.
+  solve_cert (cert1 D B [1;0;1;0] [1;1;0;1] 0 0).
+Qed.
+
+Definition tm56 := Eval compute in (TM_from_str "1RB0RE_0RC1RB_1LD0RD_1LA1RF_1LD0LE_---0LB").
+Lemma nonhalt56: ~halts tm56 c0.
+Proof.
+  solve_cert (cert1 D B [1;0;1;0] [1;1;0;1] 0 0).
+Qed.
+
+Definition tm57 := Eval compute in (TM_from_str "1RB0RE_0RC1RF_1LD0RD_1LA1RE_---0LF_1LD1RB").
+Lemma nonhalt57: ~halts tm57 c0.
+Proof.
+  solve_cert (cert1 D F [1;0;1;0] [1;1;0;1] 0 0).
+Qed.
+
+Definition tm58 := Eval compute in (TM_from_str "1RB0RF_1LC1RB_1LA1RD_---0RE_0LF0RC_0RB0LB").
+Lemma nonhalt58: ~halts tm58 c0.
+Proof.
+  solve_cert (cert1 C B [1;0;1;0] [1;1;0;1] 0 0).
+Qed.
+
+Definition tm59 := Eval compute in (TM_from_str "1RB1LF_1LC0LF_0LE1RD_---0RB_1RA1LC_0RE0RC").
+Lemma nonhalt59: ~halts tm59 c0.
+Proof.
+  solve_cert (cert1 C B [1;0;1;0] [1;1;0;1] 0 0).
+Qed.
+
+Definition tm60 := Eval compute in (TM_from_str "1RB0RE_0RC1RB_1LD0RD_1LA1RE_---0LF_0LB1RF").
+Lemma nonhalt60: ~halts tm60 c0.
+Proof.
+  solve_cert (cert1 B B [0;0;1;0] [1;1;0;1] 0 0).
+Qed.
+
+Definition tm61 := Eval compute in (TM_from_str "1RB0RF_0LC1RB_0RD1RC_1LE0RE_1LA1RF_---0LB").
+Lemma nonhalt61: ~halts tm61 c0.
+Proof.
+  solve_cert (cert1 C B [0;0;1;0] [1;1;0;1] 0 0).
+Qed.
+
+Definition tm62 := Eval compute in (TM_from_str "1RB---_0RC1RB_1LD0RD_0LE0RF_1RA1LD_---0LA").
+Lemma nonhalt62: ~halts tm62 c0.
+Proof.
+  solve_cert (cert1 D B [1;0;1;0] [1;1;0;1] 0 0).
+Qed.
+
+Definition tm63 := Eval compute in (TM_from_str "1RB---_0RC1RB_1LD0RD_0LE1RF_1RA1LD_---0LB").
+Lemma nonhalt63: ~halts tm63 c0.
+Proof.
+  solve_cert (cert1 D B [1;0;1;0] [1;1;0;1] 0 0).
+Qed.
+
+Definition tm64 := Eval compute in (TM_from_str "1RB---_0RC1RB_1LD0RD_0LE1RF_0RF1LD_1LA0LB").
+Lemma nonhalt64: ~halts tm64 c0.
+Proof.
+  solve_cert (cert1 D B [1;0;1;0] [1;1;0;1] 0 0).
+Qed.
+
+Definition tm65 := Eval compute in (TM_from_str "1RB1RA_0RC0LA_1LD0RD_0LE1RF_1RA1LD_---0RC").
+Lemma nonhalt65: ~halts tm65 c0.
+Proof.
+  solve_cert (cert1 D B [1;0;1;0] [1;1;0;1] 0 0).
+Qed.
+
+Definition tm66 := Eval compute in (TM_from_str "1RB1RA_1LC0LA_0LF1RD_---0RE_1LC0RC_1RA1LC").
+Lemma nonhalt66: ~halts tm66 c0.
+Proof.
+  solve_cert (cert1 C B [1;0;1;0] [1;1;0;1] 0 0).
+Qed.
+
+Definition tm67 := Eval compute in (TM_from_str "1RB0LB_0RC1RB_1LD0RD_1LE0RF_1RB1RF_---0LA").
+Lemma nonhalt67: ~halts tm67 c0.
+Proof.
+  solve_cert (cert1 B B [0;0;1;0] [1;1;0;1] 0 0).
+Qed.
+
+Definition tm68 := Eval compute in (TM_from_str "1RB0LB_1LC1RB_1LF1RD_---0RE_1LC0RC_1RB0RA").
+Lemma nonhalt68: ~halts tm68 c0.
+Proof.
+  solve_cert (cert1 C B [1;0;1;0] [1;1;0;1] 0 0).
+Qed.
+
+Definition tm69 := Eval compute in (TM_from_str "1RB0LB_1LC0RC_1LE1RD_---0RB_1RF0RA_0RB1RF").
+Lemma nonhalt69: ~halts tm69 c0.
+Proof.
+  solve_cert (cert1 C F [1;0;1;0] [1;1;0;1] 0 0).
+Qed.
+
+Definition tm70 := Eval compute in (TM_from_str "1RB0LB_1LC0RC_1LE1RD_---0RB_1RF0RA_1LC1RF").
+Lemma nonhalt70: ~halts tm70 c0.
+Proof.
+  solve_cert (cert1 C F [1;0;1;0] [1;1;0;1] 0 0).
+Qed.
+
+Definition tm71 := Eval compute in (TM_from_str "1LB0LB_1RC1LD_0RA1LD_0LB1RE_---0RF_1LD0RD").
+Lemma nonhalt71: ~halts tm71 c0.
+Proof.
+  solve_cert (cert1 D A [1;0;1;0] [0;1;0;1] 0 0).
+Qed.
+
+Definition tm72 := Eval compute in (TM_from_str "1LB0LB_1RC1LE_0RA0RD_1LE0RE_0LB1RF_---0RD").
+Lemma nonhalt72: ~halts tm72 c0.
+Proof.
+  solve_cert (cert1 E A [1;0;1;0] [0;1;0;1] 0 0).
+Qed.
+
+Definition tm73 := Eval compute in (TM_from_str "1RB1RB_0RC1RB_1LD0RD_0LE1RF_1RA1LD_---0LA").
+Lemma nonhalt73: ~halts tm73 c0.
+Proof.
+  solve_cert (cert1 D B [1;0;1;0] [1;1;0;1] 0 0).
+Qed.
+
+Definition tm74 := Eval compute in (TM_from_str "1RB0LC_0RC1RB_1LD0RD_1LE1RF_1RB0RA_---0RC").
+Lemma nonhalt74: ~halts tm74 c0.
+Proof.
+  solve_cert (cert1 D B [1;0;1;0] [1;1;0;1] 0 0).
+Qed.
+
+Definition tm75 := Eval compute in (TM_from_str "1RB0RC_0RC1RB_1LD0RD_0LE0RF_1RA1LD_---1LE").
+Lemma nonhalt75: ~halts tm75 c0.
+Proof.
+  solve_cert (cert1 D B [1;0;1;0] [1;1;0;1] 0 0).
+Qed.
+
+Definition tm76 := Eval compute in (TM_from_str "1RB0LD_1LC0RC_1LF1RD_---0LE_0RB1RE_1RE1RA").
+Lemma nonhalt76: ~halts tm76 c0.
+Proof.
+  solve_cert (cert1 E E [0;0;1;0] [1;1;0;1] 0 0).
+Qed.
+
+Definition tm77 := Eval compute in (TM_from_str "1RB1RD_0RC1RB_1LD0RF_1LA0LE_---0LB_1LA1RE").
+Lemma nonhalt77: ~halts tm77 c0.
+Proof.
+  solve_cert (cert1 B B [0;0;1;0] [1;1;0;1] 0 0).
+Qed.
+
+Definition tm78 := Eval compute in (TM_from_str "1RB1RD_0RC1RB_1LD0RF_0LE0LA_---1LF_1LA0RD").
+Lemma nonhalt78: ~halts tm78 c0.
+Proof.
+  solve_cert (cert1 F B [1;0;1;0] [1;1;0;1] 0 0).
+Qed.
+
+Definition tm79 := Eval compute in (TM_from_str "1RB0LE_1LC1RB_1LF1RD_---0RE_1LC0RC_1RB0RA").
+Lemma nonhalt79: ~halts tm79 c0.
+Proof.
+  solve_cert (cert1 C B [1;0;1;0] [1;1;0;1] 0 0).
+Qed.
+
+Definition tm80 := Eval compute in (TM_from_str "1RB0RE_0RC1RB_1LD0RD_1LA1RE_---0LF_0LB1RB").
+Lemma nonhalt80: ~halts tm80 c0.
+Proof.
+  solve_cert (cert1 B B [0;0;1;0] [1;1;0;1] 0 0).
+Qed.
+
+Definition tm81 := Eval compute in (TM_from_str "1RB0RE_0RC1RB_1LD0RD_1LA0RF_0LB0LE_---0LA").
+Lemma nonhalt81: ~halts tm81 c0.
+Proof.
+  solve_cert (cert1 B B [0;0;1;0] [1;1;0;1] 0 0).
+Qed.
+
+Definition tm82 := Eval compute in (TM_from_str "1RB0RE_0RC1RB_1LD0RD_1LA1RF_---0LC_---0RC").
+Lemma nonhalt82: ~halts tm82 c0.
+Proof.
+  solve_cert (cert1 D B [1;0;1;0] [1;1;0;1] 0 0).
+Qed.
+
+Definition tm83 := Eval compute in (TM_from_str "1RB0RE_0RC1RB_1LD0RD_1LA1RF_0LB0LE_---0LB").
+Lemma nonhalt83: ~halts tm83 c0.
+Proof.
+  solve_cert (cert1 B B [0;0;1;0] [1;1;0;1] 0 0).
+Qed.
+
+Definition tm84 := Eval compute in (TM_from_str "1RB0RE_0RC1RB_1LD0RD_1LA1RF_0LB0LE_---0RC").
+Lemma nonhalt84: ~halts tm84 c0.
+Proof.
+  solve_cert (cert1 B B [0;0;1;0] [1;1;0;1] 0 0).
+Qed.
+
+Definition tm85 := Eval compute in (TM_from_str "1RB0RE_0RC1RB_1LD0RD_1LA1RF_1LD0LE_---0RC").
+Lemma nonhalt85: ~halts tm85 c0.
+Proof.
+  solve_cert (cert1 D B [1;0;1;0] [1;1;0;1] 0 0).
+Qed.
+
+Definition tm86 := Eval compute in (TM_from_str "1RB1RE_0RC1RB_1LD0RD_1LA1RF_---0LF_---0LB").
+Lemma nonhalt86: ~halts tm86 c0.
+Proof.
+  solve_cert (cert1 B B [0;0;1;0] [1;1;0;1] 0 0).
+Qed.
+
+Definition tm87 := Eval compute in (TM_from_str "1RB0LF_0RC1RB_1LD0RD_1LE1RF_1RB1RA_---0LB").
+Lemma nonhalt87: ~halts tm87 c0.
+Proof.
+  solve_cert (cert1 B B [0;0;1;0] [1;1;0;1] 0 0).
+Qed.
+
+Definition tm88 := Eval compute in (TM_from_str "1RB0LF_1LC0RC_1LE1RD_---0RB_1RF0RA_1LC1RF").
+Lemma nonhalt88: ~halts tm88 c0.
+Proof.
+  solve_cert (cert1 C F [1;0;1;0] [1;1;0;1] 0 0).
+Qed.
+
+Definition tm89 := Eval compute in (TM_from_str "1RB0RF_0LC1RC_0RD1RC_1LE0RE_1LA1RF_---0LB").
+Lemma nonhalt89: ~halts tm89 c0.
+Proof.
+  solve_cert (cert1 C C [0;0;1;0] [1;1;0;1] 0 0).
+Qed.
+
+Definition tm90 := Eval compute in (TM_from_str "1RB0RF_1LC1RB_1LA1RD_---0RE_1LC0RC_---0LB").
+Lemma nonhalt90: ~halts tm90 c0.
+Proof.
+  solve_cert (cert1 C B [1;0;1;0] [1;1;0;1] 0 0).
+Qed.
+
+Definition tm91 := Eval compute in (TM_from_str "1RB0RF_1LC1RB_1LA1RD_---0RE_1LC0RC_---0LE").
+Lemma nonhalt91: ~halts tm91 c0.
+Proof.
+  solve_cert (cert1 C B [1;0;1;0] [1;1;0;1] 0 0).
+Qed.
+
+Definition tm92 := Eval compute in (TM_from_str "1RB0RF_1LC1RB_1LA1RD_---0RE_1LC0RC_1LC0LF").
+Lemma nonhalt92: ~halts tm92 c0.
+Proof.
+  solve_cert (cert1 C B [1;0;1;0] [1;1;0;1] 0 0).
+Qed.
+
+Definition tm93 := Eval compute in (TM_from_str "1RB0RF_1LC1RB_1LA1RD_---0RE_1LF0RC_1LA0LB").
+Lemma nonhalt93: ~halts tm93 c0.
+Proof.
+  solve_cert (cert1 C B [1;0;1;0] [1;1;0;1] 0 0).
+Qed.
+
+Definition tm94 := Eval compute in (TM_from_str "1RB0RF_1LC1RB_0LE0RD_---1LE_1RA1LC_1LC0RC").
+Lemma nonhalt94: ~halts tm94 c0.
+Proof.
+  solve_cert (cert1 C B [1;0;1;0] [1;1;0;1] 0 0).
+Qed.
+
+Definition tm95 := Eval compute in (TM_from_str "1RB---_0RC1RB_1LD0RD_0LE0RF_1RA0LB_---0LA").
+Lemma nonhalt95: ~halts tm95 c0.
+Proof.
+  solve_cert (cert1 B B [0;0;1;0] [1;1;0;1] 0 0).
+Qed.
+
+Definition tm96 := Eval compute in (TM_from_str "1RB---_0RC1RB_1LD0RD_0LE1RF_1RA0LB_---0LB").
+Lemma nonhalt96: ~halts tm96 c0.
+Proof.
+  solve_cert (cert1 B B [0;0;1;0] [1;1;0;1] 0 0).
+Qed.
+
+Definition tm97 := Eval compute in (TM_from_str "1RB---_0RC1RB_1LD0RD_0LE1RF_1RA0LB_---0RC").
+Lemma nonhalt97: ~halts tm97 c0.
+Proof.
+  solve_cert (cert1 B B [0;0;1;0] [1;1;0;1] 0 0).
+Qed.
+
+Definition tm98 := Eval compute in (TM_from_str "1RB---_0RC1RB_1LD0RD_0LE1RF_0RF0LB_1LA0LB").
+Lemma nonhalt98: ~halts tm98 c0.
+Proof.
+  solve_cert (cert1 B B [0;0;1;0] [1;1;0;1] 0 0).
+Qed.
+
+Definition tm99 := Eval compute in (TM_from_str "1RB---_0RC1RB_1LD0RD_0LE1RF_0RF0LB_1LA0RC").
+Lemma nonhalt99: ~halts tm99 c0.
+Proof.
+  solve_cert (cert1 B B [0;0;1;0] [1;1;0;1] 0 0).
+Qed.
+
+Definition tm100 := Eval compute in (TM_from_str "1RB---_0RC1RB_1LD0RD_0LE1RF_0RF1LD_1LA0RC").
+Lemma nonhalt100: ~halts tm100 c0.
+Proof.
+  solve_cert (cert1 D B [1;0;1;0] [1;1;0;1] 0 0).
+Qed.
+
+Definition tm101 := Eval compute in (TM_from_str "1RB---_1LC1RB_0LF1RD_---0RE_1LC0RC_1RA1LC").
+Lemma nonhalt101: ~halts tm101 c0.
+Proof.
+  solve_cert (cert1 C B [1;0;1;0] [1;1;0;1] 0 0).
+Qed.
+
+Definition tm102 := Eval compute in (TM_from_str "1RB---_1LC1RB_0LF1RD_1LA0RE_1LC0RC_0RD1LC").
+Lemma nonhalt102: ~halts tm102 c0.
+Proof.
+  solve_cert (cert1 C B [1;0;1;0] [1;1;0;1] 0 0).
+Qed.
+
+Definition tm103 := Eval compute in (TM_from_str "1RB0LB_0RC1RB_1LD0RD_0LE0RF_1RA0LB_---1LE").
+Lemma nonhalt103: ~halts tm103 c0.
+Proof.
+  solve_cert (cert1 B B [0;0;1;0] [1;1;0;1] 0 0).
+Qed.
+
+Definition tm104 := Eval compute in (TM_from_str "1RB1RB_0RC1RB_1LD0RD_0LE1RF_1RA0LB_---0LA").
+Lemma nonhalt104: ~halts tm104 c0.
+Proof.
+  solve_cert (cert1 B B [0;0;1;0] [1;1;0;1] 0 0).
+Qed.
+
+Definition tm105 := Eval compute in (TM_from_str "1RB0RC_0RC1RB_1LD0RD_0LE0RF_1RA0LB_---1LE").
+Lemma nonhalt105: ~halts tm105 c0.
+Proof.
+  solve_cert (cert1 B B [0;0;1;0] [1;1;0;1] 0 0).
+Qed.
+
+Definition tm106 := Eval compute in (TM_from_str "1RB1RC_0LA1RB_1LD0RD_0LF1RE_---0RC_1RA1LD").
+Lemma nonhalt106: ~halts tm106 c0.
+Proof.
+  solve_cert (cert1 D B [1;0;1;0] [1;1;0;1] 0 0).
+Qed.
+
+Definition tm107 := Eval compute in (TM_from_str "1RB1RC_1LA1RB_---0RD_1LE0RE_0LF1RC_1RA1LE").
+Lemma nonhalt107: ~halts tm107 c0.
+Proof.
+  solve_cert (cert1 E B [1;0;1;0] [1;1;0;1] 0 0).
+Qed.
+
+Definition tm108 := Eval compute in (TM_from_str "1RB1RC_1LA1RB_---0RD_1LE0RE_0LF1RC_0RB1LE").
+Lemma nonhalt108: ~halts tm108 c0.
+Proof.
+  solve_cert (cert1 E B [1;0;1;0] [1;1;0;1] 0 0).
+Qed.
+
+Definition tm109 := Eval compute in (TM_from_str "1RB1RC_1LA1RB_1RA1LD_0LC1RE_---0RF_1LD0RD").
+Lemma nonhalt109: ~halts tm109 c0.
+Proof.
+  solve_cert (cert1 D B [1;0;1;0] [1;1;0;1] 0 0).
+Qed.
+
+Definition tm110 := Eval compute in (TM_from_str "1RB1RC_1LA1RB_0RB1LD_0LC1RE_---0RF_1LD0RD").
+Lemma nonhalt110: ~halts tm110 c0.
+Proof.
+  solve_cert (cert1 D B [1;0;1;0] [1;1;0;1] 0 0).
+Qed.
+
+Definition tm111 := Eval compute in (TM_from_str "1RB0RE_1RC1RB_1LD0LA_---0LE_0RF0LB_1LA0RC").
+Lemma nonhalt111: ~halts tm111 c0.
+Proof.
+  solve_cert (cert1 B B [0;0;1;0] [1;1;0;1] 0 0).
+Qed.
+
+Definition tm112 := Eval compute in (TM_from_str "1RB1RE_0RC1RB_1LD0RD_0LE1RF_1RA0LB_---1LA").
+Lemma nonhalt112: ~halts tm112 c0.
+Proof.
+  solve_cert (cert1 B B [0;0;1;0] [1;1;0;1] 0 0).
+Qed.
+
+Definition tm113 := Eval compute in (TM_from_str "1RB0RF_0RC1RB_1LD1RA_0LE0RB_1RA0LB_---0LC").
+Lemma nonhalt113: ~halts tm113 c0.
+Proof.
+  solve_cert (cert1 B B [0;0;1;0] [1;1;0;1] 0 0).
+Qed.
+
+Definition tm114 := Eval compute in (TM_from_str "1RB---_0RC1RB_1LD0RD_0LE1RF_1RA1LD_---0RC").
+Lemma nonhalt114: ~halts tm114 c0.
+Proof.
+  solve_cert (cert1 D B [1;0;1;0] [1;1;0;1] 0 0).
+Qed.
+
+
+
